proofs/cam-forth/src/forth_tests.lean
@@ -1,6 +1,13 @@
 import forth
 import utils
 
+open except
+open forth_program
+open forth_vm
 open forth_word
 
-#eval 0 then (λ x, nat.succ x)
+def print_eight : forth_program := new [lit 8, print]
+
+#reduce run 2 print_eight
+-- TODO
+-- example : run 2 print_eight = ok (some [8]) := rfl
